theories/class_instances.v
@@ -10,3 +10,14 @@ Proof. apply decode_encode_instrW_inv. Qed.
 Instance DecodeInstrL_encode `{MachineParameters} (i: instr) :
   DecodeInstrL (encodeInstrWL i) i.
 Proof. apply decode_encode_instrLW_inv. Qed.
+
+#[global] Instance VersionEqSame (v : Version) : VersionEq v v true.
+Proof. constructor. Qed.
+
+#[global] Instance VersionEq_offset_cbv (v : Version) z z' :
+  CbvTC z z' →
+  VersionEq (v + z) (v + z') true.
+Proof. intros ->. constructor. Qed.
+
+#[global] Instance VersionEq_default_neq (v v' : Version) : VersionEq v v' false | 100.
+Proof. inversion 1. Qed.
